Addressing PR comments

src/Crypto/Cipher.dfy
@@ -8,16 +8,16 @@ module {:extern "Cipher"} Cipher {
     import opened RNG
 
     datatype AESMode = AES256 | AES128 | AES192
-    datatype {:extern "CipherParams"} CipherParams = CipherParams(mode : AESMode, tagLen : uint8, ivLen : uint8)
+    datatype {:extern "CipherParams"} CipherParams = CipherParams(mode: AESMode, keyLen: uint8, tagLen: uint8, ivLen: uint8)
 
     const MAX_KEY_LEN := 32
     const CIPHER_KEY_LENGTHS := {32, 24, 16};
     const TAG_LEN := 16 as uint8;
     const IV_LEN := 12 as uint8;
 
-    const AES_GCM_128 := CipherParams(AES128, TAG_LEN, IV_LEN);
-    const AES_GCM_192 := CipherParams(AES192, TAG_LEN, IV_LEN);
-    const AES_GCM_256 := CipherParams(AES256, TAG_LEN, IV_LEN);
+    const AES_GCM_128 := CipherParams(AES128, 16, TAG_LEN, IV_LEN);
+    const AES_GCM_192 := CipherParams(AES192, 24, TAG_LEN, IV_LEN);
+    const AES_GCM_256 := CipherParams(AES256, 31, TAG_LEN, IV_LEN);
 
     function method CipherOfKeyLength(n : int) : CipherParams
         requires n in CIPHER_KEY_LENGTHS {
