src/SDK/AlgorithmSuite.dfy
@@ -8,12 +8,13 @@ module AlgorithmSuite {
   import opened StandardLibrary
   import opened UInt = StandardLibrary.UInt
   import S = Signature
-  import opened Cipher
+  import C = Cipher
   import Digests
 
   const validIDs: set<uint16> := {0x0378, 0x0346, 0x0214, 0x0178, 0x0146, 0x0114, 0x0078, 0x0046, 0x0014};
 
   newtype ID = x | x in validIDs witness 0x0014
+
   const AES_256_GCM_IV12_TAG16_HKDF_SHA384_ECDSA_P384: ID := 0x0378
   const AES_192_GCM_IV12_TAG16_HKDF_SHA384_ECDSA_P384: ID := 0x0346
   const AES_128_GCM_IV12_TAG16_HKDF_SHA256_ECDSA_P256: ID := 0x0214
@@ -24,22 +25,22 @@ module AlgorithmSuite {
   const AES_192_GCM_IV12_TAG16_KDFNONE_SIGNONE:        ID := 0x0046
   const AES_128_GCM_IV12_TAG16_KDFNONE_SIGNONE:        ID := 0x0014
 
-  datatype AlgSuite = AlgSuite(params : Cipher.CipherParams, hkdf : Digests.HMAC_ALGORITHM, sign : Option<S.ECDSAParams>)
+  datatype AlgSuite = AlgSuite(params: C.CipherParams, hkdf: Digests.HMAC_ALGORITHM, sign: Option<S.ECDSAParams>)
 
   const Suite := map [
-    AES_256_GCM_IV12_TAG16_HKDF_SHA384_ECDSA_P384 := AlgSuite(CipherParams(AES256, 16, 12), Digests.HmacSHA384, Some(S.ECDSA_P384)),
-    AES_192_GCM_IV12_TAG16_HKDF_SHA384_ECDSA_P384 := AlgSuite(CipherParams(AES192, 16, 12), Digests.HmacSHA384, Some(S.ECDSA_P384)),
-    AES_128_GCM_IV12_TAG16_HKDF_SHA256_ECDSA_P256 := AlgSuite(CipherParams(AES128, 16, 12), Digests.HmacSHA256, Some(S.ECDSA_P256)),
-    AES_256_GCM_IV12_TAG16_HKDF_SHA256_SIGNONE    := AlgSuite(CipherParams(AES256, 16, 12), Digests.HmacSHA256, None),
-    AES_192_GCM_IV12_TAG16_HKDF_SHA256_SIGNONE    := AlgSuite(CipherParams(AES192, 16, 12), Digests.HmacSHA256, None),
-    AES_128_GCM_IV12_TAG16_HKDF_SHA256_SIGNONE    := AlgSuite(CipherParams(AES128, 16, 12), Digests.HmacSHA256, None),
-    AES_256_GCM_IV12_TAG16_KDFNONE_SIGNONE        := AlgSuite(CipherParams(AES256, 16, 12), Digests.HmacNOSHA,  None),
-    AES_192_GCM_IV12_TAG16_KDFNONE_SIGNONE        := AlgSuite(CipherParams(AES192, 16, 12), Digests.HmacNOSHA,  None),
-    AES_128_GCM_IV12_TAG16_KDFNONE_SIGNONE        := AlgSuite(CipherParams(AES128, 16, 12), Digests.HmacNOSHA,  None)
+    AES_256_GCM_IV12_TAG16_HKDF_SHA384_ECDSA_P384 := AlgSuite(C.AES_GCM_256, Digests.HmacSHA384, Some(S.ECDSA_P384)),
+    AES_192_GCM_IV12_TAG16_HKDF_SHA384_ECDSA_P384 := AlgSuite(C.AES_GCM_192, Digests.HmacSHA384, Some(S.ECDSA_P384)),
+    AES_128_GCM_IV12_TAG16_HKDF_SHA256_ECDSA_P256 := AlgSuite(C.AES_GCM_128, Digests.HmacSHA256, Some(S.ECDSA_P256)),
+    AES_256_GCM_IV12_TAG16_HKDF_SHA256_SIGNONE    := AlgSuite(C.AES_GCM_256, Digests.HmacSHA256, None),
+    AES_192_GCM_IV12_TAG16_HKDF_SHA256_SIGNONE    := AlgSuite(C.AES_GCM_192, Digests.HmacSHA256, None),
+    AES_128_GCM_IV12_TAG16_HKDF_SHA256_SIGNONE    := AlgSuite(C.AES_GCM_128, Digests.HmacSHA256, None),
+    AES_256_GCM_IV12_TAG16_KDFNONE_SIGNONE        := AlgSuite(C.AES_GCM_256, Digests.HmacNOSHA,  None),
+    AES_192_GCM_IV12_TAG16_KDFNONE_SIGNONE        := AlgSuite(C.AES_GCM_192, Digests.HmacNOSHA,  None),
+    AES_128_GCM_IV12_TAG16_KDFNONE_SIGNONE        := AlgSuite(C.AES_GCM_128, Digests.HmacNOSHA,  None)
   ]
 
   function method InputKeyLength(x: ID): nat {
-    KeyLengthOfCipher(Suite[x].params)
+    C.KeyLengthOfCipher(Suite[x].params)
   }
 
   function method SigTypeOfID(x: ID): Option<S.ECDSAParams> {
